Lib.v
@@ -1,0 +1,35 @@
+(** vectors and various lemmas *)
+Set Implicit Arguments.
+Unset Strict Implicit.
+Unset Printing Implicit Defensive.
+(* Vec {A} B l is a B-list of the same size as l *)
+Inductive Vec {A : Type} (B : Type) : list A -> Type :=
+    NilV : Vec B nil
+  | ConsV : forall a lA, B -> Vec B lA -> Vec B (a :: lA).
+
+Definition Vec_map {A B C : Type}(f : A -> B -> C) :=
+  fix rec (l : list A) (v : Vec B l) : Vec C l :=
+  match v with
+    NilV _ => NilV _
+  | ConsV a b lB => ConsV a (f a b) (rec _ lB)
+    end.
+
+Lemma vec_map_map {A B C D : Type}(f : A -> B -> C) (g : A -> C -> D) {l : list A}
+      (v : Vec B l) : Vec_map g (Vec_map f v) = Vec_map (fun a b => g a (f a b)) v.
+  induction v; cbn; congruence.
+Qed.
+
+Definition vec_map_fun_ext {A B C : Type}(f g : A -> B -> C) {l : list A}
+      (v : Vec B l) (h : forall a b, f a b = g a b): Vec_map f v = Vec_map g v.
+  induction v; cbn; congruence.
+Defined.
+
+Lemma commutes_if {A B : Type}(f : A -> B)(b : bool) x y :
+  (if b then f x else f y) = f (if b then x else y).
+Proof.
+destruct b; reflexivity.
+Qed.
+Lemma if_if {A : Type}(b : bool) (x y z : A) :
+  (if b then if b then x else y else z) = (if b then x else z).
+  destruct b ; reflexivity.
+Qed.
