syntaxdb.v
@@ -1,0 +1,596 @@
+
+Require Import Arith.
+Require Import Basics.
+Require Import micromega.Lia.
+
+Open Scope program_scope.
+Open Scope list_scope.
+
+Require Import Lib.
+
+Set Implicit Arguments.
+Unset Strict Implicit.
+Unset Printing Implicit Defensive.
+
+
+(* substitution in a model *)
+Reserved Notation "x [ s ]" (at level 30).
+(* substitution in the syntax *)
+Reserved Notation "x [ s ]ₛ" (at level 30).
+ (* for composition *)
+
+Declare Scope signature_scope.
+
+Record signature :=
+  { O  : Type;
+    ar : O -> list nat}.
+
+Arguments O _%signature_scope.
+
+Definition sum_of_signatures (S1 : signature)(S2 : signature) : signature :=
+  {| O := O S1 + O S2 ;
+     ar := fun o =>
+             match o with
+               inl o' => ar o'
+               | inr o' => ar o'
+               end
+  |}.
+
+Infix "+"  := sum_of_signatures : signature_scope.
+
+Inductive O_LC := App | Abs.
+
+Definition signature_LC : signature :=
+  {| O := O_LC;
+     ar := fun o => match o with
+                   App => 0 :: 0 :: nil
+                 | Abs => 1 :: nil
+                 end
+  |}.
+
+
+
+Inductive Z (S : signature) : Type :=
+  Var : nat -> Z S
+| Op : forall (o : O S), Vec (Z S) (ar o) (* this is Z^(length ar) *) -> Z S.
+
+Arguments Z S%signature_scope.
+Arguments Op [S] o.
+
+
+
+
+(* shifts on renamings *)
+Definition shiftₙ (n : nat) (f : nat -> nat)  : nat -> nat :=
+    fun p => if p <? n then p else f (p - n) + n.
+
+
+(* shifts on substitution using renamings *)
+Definition shiftₙₛ {X : Type}(var : nat -> X)(ren : (nat -> nat) -> (X -> X))(n : nat) (f : nat -> X)  : nat -> X :=
+    fun p => if p <? n then var p else ren (fun x => x + n) (f (p - n)).
+
+(* shifts on substitution using substitution structure *)
+Definition shiftₛ {X : Type}(var : nat -> X)(subst : (nat -> X) -> (X -> X))(n : nat) (f : nat -> X)  : nat -> X :=
+  shiftₙₛ var (fun f => subst (fun n => var (f n))) n f.
+
+
+Lemma shiftₙₛ_natural
+      {X : Type} (varX : nat -> X) (renX : (nat -> nat) -> (X -> X))
+      {Y : Type} (varY : nat -> Y) (renY : (nat -> nat) -> (Y -> Y))
+      (g : X -> Y)(gvar : forall n, g (varX n) = varY n)
+        (gren : forall f x, g (renX f x) = renY f (g x))
+      (n : nat) (f : nat -> X) x :
+  g (shiftₙₛ varX renX n f x) = shiftₙₛ varY renY n (fun n => g (f n)) x.
+Proof.
+  unfold shiftₙ, shiftₙₛ.
+  rewrite <- gvar, <- gren.
+  symmetry.
+  apply commutes_if.
+Qed.
+
+Lemma var_shiftₙ 
+      {X : Type}(var : nat -> X)(ren : (nat -> nat) -> (X -> X))
+      (eq_ren : forall f n, ren f (var n) = var (f n))
+      (n : nat) (f : nat -> nat) (x : nat) :
+  var ((shiftₙ n f) x) = shiftₙₛ var ren n (fun p => var (f p)) x.
+Proof.
+  unfold shiftₙ.
+  etransitivity; revgoals.
+  eapply  (shiftₙₛ_natural (g := var)).
+  - reflexivity.
+  - symmetry.
+    apply eq_ren.
+  - reflexivity.
+Qed.
+  
+Lemma shiftₙₛ_ext {X : Type}(var : nat -> X)(ren ren' : (nat -> nat) -> (X -> X))
+      (ren_eq : forall f x, ren f x = ren' f x)
+      (n : nat) (f g : nat -> X)
+      (fg_eq : forall p, f p = g p) p : shiftₙₛ var ren n f p = 
+                                   shiftₙₛ var ren' n g p .
+Proof.
+  unfold shiftₙₛ.
+  rewrite fg_eq, ren_eq.
+  reflexivity.
+Qed.
+
+(** Renaming *)
+Fixpoint Z_ren {S : signature}  (f : nat -> nat) (x : Z S) {struct x} : Z S :=
+  match x with
+    Var _ n => Var _ (f n)
+  | Op op  v => Op op (Vec_map (fun n b => (Z_ren (shiftₙ n f) b))  v)
+  end.
+
+
+
+(** Substitution *)
+Fixpoint Z_subst {S : signature}  (f : nat -> Z S) (x : Z S) : Z S :=
+  match x with
+    Var _ n => f n
+  | Op op v => Op op
+                 (Vec_map 
+                    (fun n b =>
+                       (b [ shiftₙₛ (Var S) Z_ren n f ]ₛ)
+                    ) v)
+  end
+    where "t [ f ]ₛ" := (Z_subst f t).
+
+(* Instance Z_has_substitution (S : signature) : has_substitution (Z S) := Z_subst. *)
+
+
+Record model_data (S : signature) := 
+  { carrier :> Type;
+    variables : nat -> carrier;
+    ops : forall (o : O S), Vec carrier (ar o) -> carrier;
+    (* has_subst :> has_substitution carrier *)
+    substitution : (nat -> carrier) -> (carrier -> carrier)
+
+  }.
+
+Arguments ops [S m] o.
+Notation "x [ s ]" := (substitution s x).
+Notation "↑" := (shiftₛ (variables _) (substitution (m := _))).
+(* Existing Instance has_subst . *)
+
+(*
+Definition ops_subst_law {S : signature} (m : model_data S) : Type :=
+     forall (o : O S) (v : Vec m (ar o)) (f : nat -> m),
+          (ops o v) [ f ] =
+          ops o (Vec_map
+                        (fun n t =>
+                           (* substitution (shiftₛ (variables m) substitution n f)) *)
+                           (* substitution (shiftₛ (variables m) (substitution (m := m)) n f) *)
+                           t [ ↑ n f ]
+                        )
+              v).
+*)
+
+Record model_laws {S : signature}(m : model_data S) :=
+  {
+    (* fun ext for substitution *)
+    substitution_ext : forall (f g : nat -> m),  (forall n, f n = g n) -> forall x,
+                                    x [ f ] = x [ g ] ;
+    variables_subst : forall x f, (variables m x) [ f ] = f x;
+    (* operations are module morphisms *)
+    ops_subst : 
+     forall (o : O S) (v : Vec m (ar o)) (f : nat -> m),
+          (ops o v) [ f ] =
+          ops o (Vec_map
+                        (fun n t =>
+                           (* substitution (shiftₛ (variables m) substitution n f)) *)
+                           (* substitution (shiftₛ (variables m) (substitution (m := m)) n f) *)
+                           t [ ↑ n f ]
+                        )
+              v);
+
+    (* additionnal laws (not needed for initiality) : associativity of substitution *) 
+    assoc : forall (f g : nat -> m) (x : m),
+        x [ g ] [ f ] = x [ (fun n => (g n) [ f ]) ] ;
+    id_neutral : forall (x : m), x [ variables m ] = x
+  }.
+
+Record model (S : signature) :=
+  { data :> model_data S;
+    laws : model_laws data
+  }.
+
+Arguments model S%signature_scope.
+
+Record model_mor {S : signature} (X : model_data S) (Y : model_data S) :=
+  { carrier_mor :> X -> Y ;
+    variables_mor : forall n, carrier_mor (variables X n) = variables Y n ;
+    substitution_mor : forall (f : nat -> X) (x : X), carrier_mor (x [ f ]) =
+                                              (carrier_mor x) [ carrier_mor ∘ f ];
+    ops_mor : forall (o : O S)(v : Vec X (ar o)), carrier_mor (ops o v) =
+                                                         ops o (Vec_map (fun _ => carrier_mor) v)
+  
+  }.
+
+(* Z is a model *)
+
+Definition Z_model_data (S : signature) : model_data S :=
+  {|
+  carrier := Z S;
+  variables := Var S;
+  ops := @Op S;
+  substitution := Z_subst
+ |}.
+
+Fixpoint Z_subst_ext {S}(f g : nat -> Z S) (eq : forall n, f n = g n) x :
+  x [ f ]ₛ = x [ g ]ₛ.
+Proof.
+  destruct x.
+  - cbn; apply eq.
+  - cbn.
+    f_equal.
+    apply vec_map_fun_ext.
+    intros.
+    apply Z_subst_ext.
+    intro.
+    eapply shiftₙₛ_ext.
+    + reflexivity.
+    + apply eq.
+Defined.
+
+Fixpoint Z_ren_subst_eq {S} (f : nat -> nat) (x : Z S) :
+  Z_ren f x = x [ fun n => Var S (f n) ]ₛ.
+Proof.
+  destruct x.
+  - reflexivity.
+  - cbn.
+    f_equal.
+    apply vec_map_fun_ext.
+    intros.
+    rewrite Z_ren_subst_eq.
+    cbn.
+    apply Z_subst_ext.
+    intro.
+    apply var_shiftₙ.
+    reflexivity.
+Qed.
+
+
+(* Uniqueness of the renamings *)
+Fixpoint ZModel_unique_ren (S : signature) (s : (nat -> Z S) -> Z S -> Z S)
+      (s_laws : model_laws {| carrier := Z S;
+                              variables := Var S;
+                              ops := @Op S;
+                              substitution := s|}) f z {struct z} :
+    s (fun n => Var S (f n)) z = Z_ren f z.
+Proof.
+  intros.
+  destruct z.
+  - apply (variables_subst s_laws).
+  - etransitivity.
+    apply (ops_subst s_laws).
+    cbn.
+    f_equal.
+    apply vec_map_fun_ext.
+    intros.
+    etransitivity. 
+    {  apply (substitution_ext s_laws).
+       intro n.
+       etransitivity;[symmetry; apply var_shiftₙ|].
+       intros.
+       exact (variables_subst s_laws _ _).
+       reflexivity.
+    }
+    apply (ZModel_unique_ren _ _ s_laws).
+Qed.
+
+(* Uniqueness of the substitution *)
+Fixpoint ZModel_unique_subst (S : signature) (s : (nat -> Z S) -> Z S -> Z S)
+      (s_laws : model_laws {| carrier := Z S;
+                              variables := Var S;
+                              ops := @Op S;
+                              substitution := s|}) f z {struct z} :
+    s f z = z [ f ]ₛ. 
+Proof.
+  intros.
+  destruct z.
+  - apply (variables_subst s_laws).
+  - etransitivity.
+    apply (ops_subst s_laws).
+    cbn.
+    f_equal.
+    apply vec_map_fun_ext.
+    intros.
+    etransitivity.
+    apply (ZModel_unique_subst _ _ s_laws).
+    apply Z_subst_ext.
+    intro n.
+    apply shiftₙₛ_ext.
+    + apply (ZModel_unique_ren s_laws).
+    + reflexivity.
+Qed.
+
+Lemma shiftₙₛ_shiftₙ {X : Type}(var : nat -> X)(ren : (nat -> nat) -> (X -> X))(n m : nat) (f : nat -> X)g :
+  shiftₙₛ var ren n f (shiftₙ n g m) = shiftₙₛ var ren n (fun n0 : nat => f (g n0)) m.
+Proof.
+  unfold shiftₙₛ, shiftₙ.
+  cbn -[leb].
+  destruct (m <? n) eqn:e.
+  - rewrite e.
+    reflexivity.
+  - case(Nat.ltb_spec _ _).
+    + intro. exfalso. lia.
+    + intros.
+      rewrite Nat.add_sub.
+      reflexivity.
+Qed.
+
+(*
+Lemma shiftₙ_shiftₙ g f a n : 
+  (shiftₙ a g ∘ shiftₙ a f) n = shiftₙ a (g ∘ f) n.
+Proof.
+  unfold compose.
+  cbn.
+  unfold shiftₙₛ, shiftₙ.
+  destruct (n <? a) eqn:e.
+  - rewrite e.
+    reflexivity.
+  - case(Nat.ltb_spec _ _).
+    + intro. exfalso. lia.
+    + intros. f_equal.
+      f_equal.
+      lia.
+Qed.
+*)
+Fixpoint Z_ren_subst {S : signature} g f (z : Z S) :
+Z_ren g z [ f ]ₛ = z [ fun n => f (g n)  ]ₛ.
+Proof.
+  destruct z.
+  - reflexivity.
+  - cbn.
+    f_equal.
+    rewrite vec_map_map.
+    apply vec_map_fun_ext.
+    intros.
+    cbn.
+    etransitivity;[apply Z_ren_subst|].
+    apply Z_subst_ext.
+    intro n.
+    apply shiftₙₛ_shiftₙ.
+Qed.
+
+Lemma Z_ren_ren {S : signature} g f (z : Z S) :
+Z_ren g (Z_ren f z) = Z_ren (g ∘ f) z.
+  rewrite Z_ren_subst_eq at 1.
+  rewrite Z_ren_subst.
+  symmetry.
+  apply Z_ren_subst_eq.
+Qed.
+
+
+  (* Z_ren (shiftₙ a g) (shiftₙₛ (Var S) Z_ren a f n) = shiftₙₛ (Var S) Z_ren a (fun n0 : nat => Z_ren g (f n0)) n *)
+(* TODO: factoriser un principe de recurrence *)
+Fixpoint Z_subst_ren {S : signature} g f (z : Z S) :
+Z_ren g (z [ f ]ₛ) = z [ fun n => Z_ren g (f n)  ]ₛ.
+Proof.
+  destruct z.
+  - reflexivity.
+  - cbn.
+    f_equal.
+    rewrite vec_map_map.
+    apply vec_map_fun_ext.
+    intros.
+    cbn.
+    etransitivity;[apply Z_subst_ren|].
+    apply Z_subst_ext.
+    intro n.
+
+  unfold shiftₙ, shiftₙₛ.
+  cbn -[leb].
+  rewrite <- (commutes_if (Z_ren _)).
+  cbn -[leb].
+  destruct (n <? a) eqn:eqna.
+  + reflexivity.
+  + cbn -[leb].
+    rewrite Z_ren_ren.
+    rewrite Z_ren_ren.
+    rewrite 2 Z_ren_subst_eq.
+    apply Z_subst_ext.
+    intro m.
+    unfold compose.
+    cbn -[leb].
+    case(Nat.ltb_spec _ _).
+    * intro. exfalso. lia.
+    * intros. 
+      rewrite Nat.add_sub.
+      reflexivity.
+Qed.
+
+Fixpoint Z_subst_subst {S : signature}
+      (f g : nat -> Z S) (x : Z S) :
+  (x [g]ₛ) [f]ₛ = x [fun n : nat => g n [f]ₛ]ₛ.
+Proof.
+  destruct x.
+  - reflexivity.
+  - cbn.
+    f_equal.
+    rewrite vec_map_map.
+    apply vec_map_fun_ext.
+    intros.
+    cbn.
+    etransitivity;[apply Z_subst_subst|].
+    apply Z_subst_ext.
+    intro n.
+    cbn.
+    (* ca devrait marcher *)
+  unfold shiftₙ, shiftₙₛ.
+  cbn -[leb].
+  rewrite <- (commutes_if (Z_subst _)).
+  cbn -[leb].
+  rewrite if_if.
+  destruct (n <? a) eqn:eqna.
+  + reflexivity.
+  + cbn -[leb].
+    rewrite Z_ren_subst.
+    erewrite Z_subst_ext; revgoals.
+    {
+      intro.
+  - case(Nat.ltb_spec _ _).
+    + intro. exfalso. lia.
+    + intros. f_equal.
+      rewrite Nat.add_sub.
+      reflexivity.
+      }
+    symmetry.
+    apply Z_subst_ren.
+    Qed.
+
+Fixpoint Vec_map_id {A B : Type}{l : list A}(v : Vec B l) : Vec_map (fun _ x => x) v = v.
+  destruct v.
+  -  reflexivity.
+  -  cbn.
+     f_equal.
+     apply Vec_map_id.
+Defined.
+
+Lemma shiftₙ_id (n : nat) (p : nat)  : 
+  shiftₙ n (fun x => x) p = p.
+  unfold shiftₙ.
+  case (Nat.ltb_spec).
+  + reflexivity.
+  + lia.
+Qed.
+
+Lemma shiftₙₛ_var {X : Type}(var : nat -> X)ren
+      (eq_ren : forall f n, ren f (var n) = var (f n))
+      n m : shiftₙₛ var ren n var m = var m.
+Proof.
+    unshelve erewrite <- (var_shiftₙ _ _ (fun n => n)).
+    + auto.
+    + cbn.
+      f_equal.
+      apply shiftₙ_id.
+Qed.
+Fixpoint Z_subst_id {S} (z : Z S) : z [Var S ]ₛ = z.
+  destruct z.
+  - reflexivity.
+  - cbn.
+    f_equal.
+    etransitivity;[|apply Vec_map_id].
+    apply vec_map_fun_ext.
+    intros.
+    etransitivity;[|apply Z_subst_id].
+    apply Z_subst_ext.
+    intro n.
+    apply shiftₙₛ_var.
+    reflexivity.
+Qed.
+  
+
+Lemma Z_model_laws (S : signature) : model_laws (Z_model_data S).
+Proof.
+  repeat split.
+  - exact Z_subst_ext.
+  - intros o v f.
+    cbn.
+    f_equal.
+    apply vec_map_fun_ext.
+    intros.
+    apply Z_subst_ext.
+    intro.
+    unfold shiftₙₛ.
+    rewrite Z_ren_subst_eq.
+    reflexivity.
+  - apply Z_subst_subst. 
+  - apply Z_subst_id.
+Qed.
+
+
+Definition ZModel (S : signature) : model S :=
+  {| data := Z_model_data S; laws := Z_model_laws S |}.
+
+(* the initial morphism *)
+
+Fixpoint ini_mor {S : signature} (m : model_data S )(x : Z S) : m :=
+  match x with
+        Var _ n => variables _ n
+      | Op o v   => ops o (Vec_map (fun _ => ini_mor m) v)
+  end.
+
+(* the initial morphism preserves renaming *)
+Fixpoint mor_ren { S : signature}(m : model S)(f : nat -> nat) (x : Z S) :
+  ini_mor m (Z_ren f x) = (ini_mor m x) [ variables m ∘ f ].
+  destruct x as [n|o v].
+  - cbn.
+    rewrite (variables_subst (laws m)).
+    reflexivity.
+  - cbn -[leb].
+    rewrite (ops_subst (laws m)).
+    repeat rewrite vec_map_map.
+    cbn -[leb].
+    apply f_equal.
+    induction v.
+    + reflexivity.
+    + cbn -[leb].
+      f_equal; revgoals.
+      * exact IHv.
+      * cbn -[leb].
+        rewrite mor_ren.
+        cbn -[leb].
+        apply (substitution_ext (laws m)).
+        intro n.
+        unfold compose.
+        apply var_shiftₙ.
+        cbn.
+        intros.
+        rewrite (variables_subst (laws m)).
+        reflexivity.
+Defined.
+
+
+(* the initial morphism preserves substitution *)
+Fixpoint mor_subst {S : signature}(m : model S)(f : nat -> Z S) (x : Z S) :
+  (* ini_mor m (x [ f ]ₛ) = (ini_mor m x) [fun y => ini_mor m (f y)]. *)
+  ini_mor m (x [ f ]ₛ) = (ini_mor m x) [ ini_mor m ∘ f].
+  destruct x as [n|o v].
+  - cbn.
+    rewrite (variables_subst (laws m)).
+    reflexivity.
+  - cbn -[leb].
+    rewrite (ops_subst (laws m)).
+    repeat rewrite vec_map_map.
+    cbn -[leb].
+    apply f_equal.
+    induction v.
+    + reflexivity.
+    + cbn -[leb].
+      f_equal; revgoals.
+      * exact IHv.
+      * rewrite mor_subst.
+        apply (substitution_ext (laws m)).
+        intro n.
+        unfold compose.
+        apply shiftₙₛ_natural.
+        -- reflexivity.
+        -- intros.
+           apply mor_ren.
+Qed.
+
+
+
+Program Definition initial_morphism {S : signature}(m : model S) : model_mor (ZModel S) m :=
+  {|
+  carrier_mor := ini_mor m;
+  |}.
+Next Obligation.
+  apply mor_subst.
+Qed.
+
+Fixpoint initial_morphism_unique {S : signature}(m : model_data S) (f : model_mor (ZModel S) m)
+     x : f x = ini_mor m x. 
+Proof.
+  destruct x.
+  - apply variables_mor.
+  - etransitivity.
+    apply ops_mor.
+    cbn.
+    f_equal.
+    apply vec_map_fun_ext.
+    intros.
+    apply initial_morphism_unique.
+Qed.
+
