Makefile
@@ -1,0 +1,13 @@
+OBJS = Lib.vo Quot.vo syntaxdb.vo quotsyntax.vo
+CC = coqc
+
+all: $(OBJS)
+
+%.vo: %.v
+	coqc $(FLAGS) $<
+
+clean:
+	rm *.vo
+
+
+
